Etst/Subtyping/Utils/ExprClearVars.lean
@@ -1,0 +1,433 @@
+import Etst.WFC.Utils.InterpretationMono
+
+namespace Etst
+
+
+namespace Expr
+  def clearVars_eq_var
+    {ub: Nat}
+    (lt: x < ub)
+  :
+    clearVars (E := E) ub (.var x) = .var x
+  :=
+    if_pos lt
+  
+  def clearVars_eq_none
+    {ub: Nat}
+    (nlt: ¬ x < ub)
+  :
+    clearVars (E := E) ub (.var x) = none
+  :=
+    if_neg nlt
+  
+  def clearVars_none_eq_none
+  :
+    clearVars (E := E) n none = none
+  :=
+    show (if 0 < n + 1 then var 0 else none).arbUn.compl = none from
+    if_pos (Nat.zero_lt_succ n) ▸ rfl
+  
+  def clearVars_idempotent (expr: Expr E):
+    (expr.clearVars n).clearVars n = expr.clearVars n
+  :=
+    match expr with
+    | .df _ _ => rfl
+    | .var x =>
+      if h: x < n then by
+        rw [clearVars_eq_var h, clearVars_eq_var h]
+      else by
+        rw [clearVars_eq_none h]
+        exact clearVars_none_eq_none
+    | .null => rfl
+    | .pair left rite =>
+        congrArg₂ Expr.pair
+          left.clearVars_idempotent
+          rite.clearVars_idempotent
+    | .ir left rite =>
+        congrArg₂ Expr.ir
+          left.clearVars_idempotent
+          rite.clearVars_idempotent
+    | .condFull body =>
+        congrArg Expr.condFull body.clearVars_idempotent
+    | .compl body =>
+        congrArg Expr.compl body.clearVars_idempotent
+    | .arbIr body =>
+        congrArg Expr.arbIr (body.clearVars_idempotent)
+  
+  def clearVars_isClean (expr: Expr E):
+    IsClean expr.clearVars
+  :=
+    (clearVars_idempotent expr).symm
+  
+end Expr
+
+namespace SingleLaneExpr
+  open Expr
+  
+  def clearVars_preserves_interp_bv
+    (expr: SingleLaneExpr)
+    (bv bvRest: List Pair)
+    (b c: Valuation Pair)
+  :
+    Eq
+      (expr.intp2 bv b c)
+      (intp2 (expr.clearVars bv.length) (bv ++ bvRest) b c)
+  :=
+    match expr with
+    | .df _ _ => rfl
+    | .var x =>
+      if h: x < bv.length then
+        let ltExtra: x < (bv ++ bvRest).length := 
+          h.trans_le (bv.length_le_append_rite bvRest)
+        let eq: clearVars bv.length (var x) = var x :=
+          clearVars_eq_var h
+        by
+        rw [intp2_var_eq_of_lt h, eq]
+        rw [intp2_var_eq_of_lt ltExtra]
+        rw [bv.getElem_append_left h]
+      else
+        clearVars_eq_none h ▸
+        SingleLaneExpr.intp2_var_eq_empty h ▸
+        SingleLaneExpr.intp2_none_eq_empty.symm
+    | .null => rfl
+    | .pair left rite =>
+      eq_intp2_pair_of_eq
+        (clearVars_preserves_interp_bv left bv bvRest b c)
+        (clearVars_preserves_interp_bv rite bv bvRest b c)
+    | .ir left rite =>
+      eq_intp2_ir_of_eq
+        (clearVars_preserves_interp_bv left bv bvRest b c)
+        (clearVars_preserves_interp_bv rite bv bvRest b c)
+    | .condFull body =>
+      eq_intp2_condFull_of_eq
+        (clearVars_preserves_interp_bv body bv bvRest b c)
+    | .compl body =>
+      let ih := clearVars_preserves_interp_bv body bv bvRest c b
+      eq_intp2_compl_of_eq ih
+    | .arbIr body =>
+      eq_intp2_arbIr_of_eq (fun dX =>
+        clearVars_preserves_interp_bv (bvRest := bvRest) body (dX :: bv) b c)
+  
+  def clearVars_preserves_interp
+    (expr: SingleLaneExpr)
+    (bv: List Pair)
+    (b c: Valuation Pair)
+  :
+    Eq
+      (expr.intp2 [] b c)
+      (intp2 expr.clearVars bv b c)
+  :=
+    clearVars_preserves_interp_bv expr [] bv b c
+  
+  namespace IsClean
+    def var_independent
+      {expr: SingleLaneExpr}
+      (isClean: expr.IsClean)
+      (bv0 bv1: List Pair)
+      (b c: Valuation Pair)
+    :
+      expr.intp2 bv0 b c = expr.intp2 bv1 b c
+    :=
+      isClean ▸
+      clearVars_preserves_interp expr bv0 b c ▸
+      clearVars_preserves_interp expr bv1 b c ▸
+      rfl
+
+    def changeBv
+      {expr: SingleLaneExpr}
+      (isClean: IsClean expr)
+      {bv1: List Pair}
+      (dInExpr: expr.intp2 bv0 b c d)
+    :
+      expr.intp2 bv1 b c d
+    :=
+      var_independent isClean bv0 bv1 b c ▸ dInExpr
+    
+  end IsClean
+end SingleLaneExpr
+
+namespace BasicExpr
+  def clearVars_lane_comm
+    (expr: BasicExpr)
+    (lane: Set3.Lane)
+    (i: Nat := 0)
+  :
+    Eq
+      (Expr.clearVars i (expr.toLane lane))
+      (BasicExpr.toLane (Expr.clearVars i expr) lane)
+  :=
+    match expr with
+    | .df x => rfl
+    | .var x => by
+      show
+        Eq
+          (Expr.clearVars i (.var x))
+          (toLane (Expr.clearVars i (.var x)) lane)
+      if h: x < i then
+        rw [Expr.clearVars_eq_var h, Expr.clearVars_eq_var h]
+        rfl
+      else
+        rw [Expr.clearVars_eq_none h, Expr.clearVars_eq_none h]
+        rfl
+    | .null => rfl
+    | .pair left rite =>
+        congrArg₂
+          SingleLaneExpr.pair
+          (clearVars_lane_comm left lane i)
+          (clearVars_lane_comm rite lane i)
+    | .ir left rite =>
+        congrArg₂
+          SingleLaneExpr.ir
+          (clearVars_lane_comm left lane i)
+          (clearVars_lane_comm rite lane i)
+    | .condFull body =>
+        congrArg
+          SingleLaneExpr.condFull
+          (clearVars_lane_comm body lane i)
+    | .compl body =>
+        congrArg
+          SingleLaneExpr.compl
+          (clearVars_lane_comm body lane.toggle i)
+    | .arbIr body =>
+        congrArg
+          SingleLaneExpr.arbIr
+          (clearVars_lane_comm body lane (i + 1))
+  
+  def clearVars_preserves_interp
+    (expr: BasicExpr)
+    (bv: List Pair)
+    (b c: Valuation Pair)
+  :
+    expr.triIntp2 [] b c = triIntp2 expr.clearVars bv b c
+  :=
+    let eqBvDef := (expr.toLane .defLane).clearVars_preserves_interp bv b c
+    let eqBvPos := (expr.toLane .posLane).clearVars_preserves_interp bv b c
+    Set3.eq
+      (eqBvDef.trans (clearVars_lane_comm expr .defLane ▸ rfl))
+      (eqBvPos.trans (clearVars_lane_comm expr .posLane ▸ rfl))
+end BasicExpr
+
+namespace DefList
+  def interp_eq_bv
+    (dl: DefList)
+    (x: Nat)
+    (bv0 bv1: List Pair)
+    (b c: Valuation Pair)
+  :
+    (dl.getDef x).triIntp2 bv0 b c = (dl.getDef x).triIntp2 bv1 b c
+  :=
+    dl.isClean x ▸
+    BasicExpr.clearVars_preserves_interp (dl.getDef x) bv0 b c ▸
+    BasicExpr.clearVars_preserves_interp (dl.getDef x) bv1 b c ▸
+    rfl
+  
+  def interp_eq_bv_def
+    (dl: DefList)
+    (x: Nat)
+    (bv0 bv1: List Pair)
+    (b c: Valuation Pair)
+  :
+    Eq
+      (((dl.getDef x).toLane .defLane).intp2 bv0 b c)
+      (((dl.getDef x).toLane .defLane).intp2 bv1 b c)
+  :=
+    Set3.eq_def (dl.interp_eq_bv x bv0 bv1 b c)
+  
+  def interp_eq_bv_pos
+    (dl: DefList)
+    (x: Nat)
+    (bv0 bv1: List Pair)
+    (b c: Valuation Pair)
+  :
+    Eq
+      (((dl.getDef x).toLane .posLane).intp2 bv0 b c)
+      (((dl.getDef x).toLane .posLane).intp2 bv1 b c)
+  :=
+    Set3.eq_pos (dl.interp_eq_bv x bv0 bv1 b c)
+  
+end DefList
+
+namespace SingleLaneExpr
+  def InWfm.of_in_def
+    (inDef: InWfm bv dl ((dl.getDef x).toLane lane) d)
+  :
+    InWfm [] dl (.df lane x) d
+  :=
+    of_in_def_no_bv
+      (match lane with
+      | .defLane =>
+        let eqDef := dl.interp_eq_bv_def x [] bv dl.wfm dl.wfm
+        show intp2 _ _ _ _ _ from
+        eqDef ▸ inDef
+      | .posLane =>
+        let eqPos := dl.interp_eq_bv_pos x [] bv dl.wfm dl.wfm
+        show intp2 _ _ _ _ _ from
+        eqPos ▸ inDef)
+  
+  def InWfm.in_def
+    (inDef: InWfm [] dl (.df lane x) d)
+  :
+    InWfm bv dl ((dl.getDef x).toLane lane) d
+  :=
+    show intp2 _ _ _ _ _ from
+    match lane with
+    | .defLane =>
+      dl.interp_eq_bv_def x bv [] dl.wfm dl.wfm ▸
+      in_def_no_bv inDef
+    | .posLane =>
+      dl.interp_eq_bv_pos x bv [] dl.wfm dl.wfm ▸
+      in_def_no_bv inDef
+  
+end SingleLaneExpr
+
+
+namespace Expr
+  def freeVarUB
+    (expr: Expr E)
+    (depth: Nat := 0)
+  :
+    Nat
+  :=
+    match expr with
+    | .df _ _ => 0
+    | .var x => if x < depth then 0 else x + 1 - depth
+    | .null => 0
+    | .pair left rite =>
+        Nat.max (left.freeVarUB depth) (rite.freeVarUB depth)
+    | .ir left rite =>
+        Nat.max (left.freeVarUB depth) (rite.freeVarUB depth)
+    | .condFull body => body.freeVarUB depth
+    | .compl body => body.freeVarUB depth
+    | .arbIr body => body.freeVarUB depth
+  
+  def freeVarUB_pair_lt_left
+    (h : (pair l r).freeVarUB d < x)
+  :
+    l.freeVarUB d < x
+  :=
+    Nat.lt_of_le_of_lt (Nat.le_max_left _ _) h
+  
+  def freeVarUB_pair_lt_rite
+    (h : (pair l r).freeVarUB d < x)
+  :
+    r.freeVarUB d < x
+  :=
+    Nat.lt_of_le_of_lt (Nat.le_max_right _ _) h
+  
+  def freeVarUB_un_lt_left
+    (h : (un l r).freeVarUB d < x)
+  :
+    l.freeVarUB d < x
+  :=
+    Nat.lt_of_le_of_lt (Nat.le_max_left _ _) h
+  
+  def freeVarUB_un_lt_rite
+    (h : (un l r).freeVarUB d < x)
+  :
+    r.freeVarUB d < x
+  :=
+    Nat.lt_of_le_of_lt (Nat.le_max_right _ _) h
+  
+  def freeVarUB_ir_lt_left
+    (h : (ir l r).freeVarUB d < x)
+  :
+    l.freeVarUB d < x
+  :=
+    Nat.lt_of_le_of_lt (Nat.le_max_left _ _) h
+  
+  def freeVarUB_ir_lt_rite
+    (h : (ir l r).freeVarUB d < x)
+  :
+    r.freeVarUB d < x
+  :=
+    Nat.lt_of_le_of_lt (Nat.le_max_right _ _) h
+  
+  def freeVarUB_pair_le_left
+    (h : (pair l r).freeVarUB d ≤ x)
+  :
+    l.freeVarUB d ≤ x
+  :=
+    Nat.le_trans (Nat.le_max_left _ _) h
+  
+  def freeVarUB_pair_le_rite
+    (h : (pair l r).freeVarUB d ≤ x)
+  :
+    r.freeVarUB d ≤ x
+  :=
+    Nat.le_trans (Nat.le_max_right _ _) h
+  
+  def freeVarUB_un_le_left
+    (h : (un l r).freeVarUB d ≤ x)
+  :
+    l.freeVarUB d ≤ x
+  :=
+    Nat.le_trans (Nat.le_max_left _ _) h
+  
+  def freeVarUB_un_le_rite
+    (h : (un l r).freeVarUB d ≤ x)
+  :
+    r.freeVarUB d ≤ x
+  :=
+    Nat.le_trans (Nat.le_max_right _ _) h
+  
+  def freeVarUB_ir_le_left
+    (h : (ir l r).freeVarUB d ≤ x)
+  :
+    l.freeVarUB d ≤ x
+  :=
+    Nat.le_trans (Nat.le_max_left _ _) h
+  
+  def freeVarUB_ir_le_rite
+    (h : (ir l r).freeVarUB d ≤ x)
+  :
+    r.freeVarUB d ≤ x
+  :=
+    Nat.le_trans (Nat.le_max_right _ _) h
+  
+  
+  def clearVars_eq_of_ub
+    {expr: Expr E}
+    {ub: Nat}
+    (h: expr.freeVarUB ≤ ub)
+  :
+    Expr.clearVars ub expr = expr
+  :=
+    let leL {l r} (h: max l r ≤ ub) := Nat.le_trans (Nat.le_max_left l r) h
+    let leR {l r} (h: max l r ≤ ub) := Nat.le_trans (Nat.le_max_right l r) h
+    match expr with
+    | .df _ _ => rfl
+    | .var _ => clearVars_eq_var (Nat.lt_of_succ_le h)
+    | .null => rfl
+    | .pair _ _ =>
+      congrArg₂ Expr.pair
+        (clearVars_eq_of_ub (leL h))
+        (clearVars_eq_of_ub (leR h))
+    | .ir _ _ =>
+      congrArg₂ Expr.ir
+        (clearVars_eq_of_ub (leL h))
+        (clearVars_eq_of_ub (leR h))
+    | .condFull _ =>
+      congrArg Expr.condFull (clearVars_eq_of_ub h)
+    | .compl _ =>
+      congrArg Expr.compl (clearVars_eq_of_ub h)
+    | .arbIr _ =>
+      congrArg
+        Expr.arbIr
+        (clearVars_eq_of_ub (Nat.le_trans h (Nat.le_succ _)))
+end Expr
+
+namespace SingleLaneExpr
+  def intp_append
+    (dl: DefList)
+    {expr: SingleLaneExpr}
+    {bv: List Pair}
+    (h: expr.freeVarUB ≤ bv.length)
+    rest
+    (p: Pair)
+  :
+    expr.intp bv dl.wfm p ↔ expr.intp (bv ++ rest) dl.wfm p
+  := by
+    unfold SingleLaneExpr.intp
+    rw [SingleLaneExpr.clearVars_preserves_interp_bv]
+    rw [Expr.clearVars_eq_of_ub h]
+end SingleLaneExpr
